lakefile.lean
@@ -4,6 +4,7 @@ open Lake DSL
 package lean_tla
 
 require mathlib from git "https://github.com/leanprover-community/mathlib4.git"
+require cslib from git "https://github.com/leanprover/cslib" @ "main"
 
 @[default_target]
 lean_lib TlaDsl
